Review the proof about quadruples

Quadruple.v
@@ -8,348 +8,70 @@ From Rela Require Import Inliner.
 From Coq Require Import Lia.
 Import Arith.
 
-(** Function for loop inlining in Com **)
+(* (** Function for loop inlining in Com **) *)
 
-Fixpoint inliner c inline:=
-  match c with
-  | CSeq p1 p2 => CSeq (inliner p1 inline) (inliner p2 inline)
-  | CIf b p1 p2 => CIf b (inliner p1 inline) (inliner p2 inline)
-  | CWhile b p inv => inline b p inv
-  | _ => c
-  end.
-
-(** Function for recursive loop inlining in Com **)
-
-Fixpoint k_inliner n c :=
+Fixpoint unroll n b p :=
   match n with
-  | 0 => CWhile BTrue CSkip (fun _ => True)
-  | S n' => inliner c (fun b p inv =>
-                        k_inliner n' (CIf b (CSeq p (CWhile b p inv)) CSkip))
+  | 0 => CWhile BTrue CSkip (fun _ => True) (fun _ => 0)
+  | S n => CIf b  (CSeq p (unroll n b p)) CSkip
   end.
 
-(** Some fact about the inlining **)
-
-Lemma inline_cskip n : k_inliner (S n) CSkip = CSkip.
+Lemma inline_n_ceval n p b inv var s ps s':
+  ceval (unroll n b p) s ps s' -> ceval (CWhile b p inv var) s ps s'.
 Proof.
-  reflexivity.
-Qed.
-
-Lemma inline_cass n x a1: k_inliner (S n) (CAss x a1) = (CAss x a1).
-Proof.
-  reflexivity.
-Qed.
-
-Lemma inline_cassr n x a1: k_inliner (S n) (CAssr x a1) = (CAssr x a1).
-Proof.
-  reflexivity.
-Qed.
-
-Lemma inline_cassert n b: k_inliner (S n) (CAssert b) = (CAssert b).
-Proof.
-  reflexivity.
-Qed.
-
-Lemma inline_cseq n p1 p2: k_inliner (S n) (CSeq p1 p2) =
-                           CSeq (k_inliner (S n) p1) (k_inliner (S n) p2).
-Proof.
-  reflexivity.
-Qed.
-
-Lemma inline_cif n b p1 p2: k_inliner (S n) (CIf b p1 p2) =
-                            CIf b (k_inliner (S n)  p1)  (k_inliner (S n) p2).
-Proof.
-  reflexivity.
-Qed.
-
-Lemma inline_cwhile n p b inv: k_inliner (S n) (CWhile b p inv) =
-                               k_inliner n (CIf b (CSeq p (CWhile b p inv)) CSkip).
-Proof.
-  reflexivity.
-Qed.
-
-Lemma inline_ccall n f:
-  k_inliner (S n) (CCall f) = CCall f.
-Proof.
-  reflexivity.
-Qed.
-
-(* ceval is inlining insensitive on command *)
-
-Definition inl b p inv := CIf b (CSeq p (CWhile b p inv)) CSkip.
-
-Lemma ceval_inline p s ps s':
-  ceval p s ps s' -> ceval (inliner p inl) s ps s'.
-Proof.
-  intros.
-  induction H.
-  + apply E_Skip.
-  + apply E_Ass.
-    all: try now auto.
-  + apply E_Assr.
-    all: try now auto.
-  + apply E_Assert.
-  + simpl. apply E_IfTrue; [now auto | now auto].
-  + simpl. apply E_IfFalse; [now auto | now auto].
-  + simpl. eapply E_Seq.
-  - apply IHceval1.
-  - apply IHceval2.
-    + simpl. unfold inl. apply E_IfFalse. now auto. apply E_Skip.
-    + simpl. unfold inl. apply E_IfTrue. now auto.
-      eapply E_Seq.
-  - apply H0.
-  - apply H1.
-    + simpl. apply E_Call. assumption.
-Qed.
-
-Lemma inline_ceval p s ps s':
-  ceval (inliner p inl) s ps s' -> ceval p s ps s'.
-Proof.
-  intros.
   generalize dependent s.
   generalize dependent s'.
-  generalize dependent ps.
-  induction p;intros.
-  + inversion H;subst.
-    apply E_Skip.
-  + inversion H;subst.
-    apply E_Ass. all: try now auto.
-  + inversion H;subst.
-    apply E_Assr. all: try now auto.
-  + inversion H;subst.
-    apply E_Assert.
-  + inversion H;subst.
-    eapply E_Seq.
-    * apply IHp1. apply H2.
-    * apply IHp2. apply H6.
-  + inversion H;subst.
-    * eapply E_IfTrue.
-      assumption.
-      apply IHp1. apply H7.
-    * eapply E_IfFalse.
-      assumption.
-      apply IHp2. apply H7.
-  + simpl in H. unfold inl in H.
-    inversion H; subst.
-    * inversion H7;subst.
-      eapply E_WhileTrue.
-      assumption.
-      apply H2.
-      apply H8.
-    * inversion H7;subst.
+  induction n.
+  * intros.
+    apply ceval_inf_loop in H.
+    contradiction H.
+  * simpl. intros.
+    inversion H;subst.
+    + inversion H7;subst.
+      eapply E_WhileTrue ;[assumption | apply H2 | ].
+      apply IHn;assumption.
+    + inversion H7;subst.
       apply E_WhileFalse.
       assumption.
-  +  simpl in H. assumption.
 Qed.
 
-(* ceval is "n" inlining insensitive on command *)
-
-Lemma inline_n_ceval n p s ps s':
-  ceval (k_inliner n p) s ps s' -> ceval p s ps s'.
-Proof.
-  generalize dependent s.
-  generalize dependent s'.
-  generalize dependent p.
-  induction n.
-  * intros.
-    apply ceval_inf_loop in H.
-    contradiction H.
-  * induction p;intros.
-  + apply H.
-  + apply H.
-  + apply H.
-  + apply H.
-  + inversion H;subst.
-    apply E_Seq with s'0.
-  - apply IHp1.
-    apply H2.
-  - apply IHp2.
-    apply H6.
-    + inversion H;subst.
-  - apply E_IfTrue.
-    ** assumption.
-    ** apply IHp1.
-       assumption.
-  - apply E_IfFalse.
-    ** assumption.
-    ** apply IHp2.
-       assumption.
-    + simpl in H.
-      destruct n.
-  -
-    simpl in H.
-    apply ceval_inf_loop in H.
-    contradiction H.
-  - apply IHn in H.
-    inversion H;subst.
-    ++ inversion H7;subst.
-       eapply E_WhileTrue.
-       assumption.
-       apply H2.
-       apply H8.
-    ++ inversion H7;subst.
-       apply E_WhileFalse.
-       assumption.
-    + simpl in H. assumption.
-Qed.
-
-Lemma inline_ceval_S n p s  s' ps:
-  ceval (k_inliner n p) s ps s' ->
-  forall m, n <= m -> ceval (k_inliner m p) s ps s'.
+Lemma inline_ceval_S n p b s ps s':
+  ceval (unroll n b p) s ps s' ->
+  forall m, n <= m -> ceval (unroll m b p) s ps s'.
 Proof.
   intros.
   generalize dependent s.
   generalize dependent s'.
-  generalize dependent p.
   generalize dependent m.
   induction n.
-  * intros.
+  - intros.
     apply ceval_inf_loop in H.
     contradiction H.
-  * destruct m as [| m].
-  + intros. inversion H0.
-  + induction p;intros.
-  - apply H.
-  - apply H.
-  - apply H.
-  - apply H.
-  - rewrite inline_cseq in H.
-    inversion H;subst.
-    rewrite inline_cseq.
-    apply E_Seq with s'0.
-    ** apply IHp1.
-       apply H3.
-    ** apply IHp2.
-       apply H7.
-  - rewrite inline_cif in H.
-    inversion H;subst.
-    ** rewrite inline_cif.
-       apply E_IfTrue.
-    ++ assumption.
-    ++ apply IHp1.
-       apply H8.
-       ** rewrite inline_cif.
-          apply E_IfFalse.
-    ++ assumption.
-    ++ apply IHp2.
-       apply H8.
-  -      simpl in H.
-         destruct n.
-         **
-           simpl in H.
-           apply ceval_inf_loop in H.
-           contradiction H.
-         ** apply (IHn m) in H.
-            apply H.
-            now apply Le.le_S_n.
-  - apply H.
+  - destruct m as [| m].
+    + intros. inversion H0.
+    + simpl; intros.
+      inversion H;subst.
+      * inversion H8;subst.
+        apply E_IfTrue;[assumption|].
+        eapply E_Seq ;[apply H3|].
+        apply IHn.
+        Lia.lia.
+        assumption.
+      * apply E_IfFalse;assumption.
 Qed.
 
-Lemma ceval_inline_n p s s' ps:
-  ceval p s ps s' -> exists n, ceval (k_inliner n p) s ps s'.
+Lemma ceval_inline_n p s s' b inv var ps:
+  ceval (CWhile b p inv var) s ps s' -> exists n, ceval (unroll n b p) s ps s'.
 Proof.
-  induction 1;intros.
+  intros.
+  remember (CWhile b p inv var) as original_command eqn:Horig.
+  induction H; inversion Horig; subst;simpl.
   * exists 1.
-    apply E_Skip.
-  * exists 1.
-    apply E_Ass.
-    all: try now auto.
-  * exists 1.
-    apply E_Assr.
-    all: try now auto.
-  * exists 1.
-    apply E_Assert.
-  * destruct IHceval as [n IH].
-    exists n.
-    destruct n.
-  - apply ceval_inf_loop in IH.
-    contradiction IH.
-  - rewrite inline_cif.
-    apply E_IfTrue.
-    assumption.
-    apply IH.
-    * destruct IHceval as [n IH].
-      exists n.
-      destruct n.
-  - apply ceval_inf_loop in IH.
-    contradiction IH.
-  - rewrite inline_cif.
-    apply E_IfFalse.
-    assumption.
-    apply IH.
-    * destruct IHceval1 as [n1 IH1].
-      destruct IHceval2 as [n2 IH2].
-      exists (max n1 n2).
-      destruct n1 as [|n1].
-    + apply ceval_inf_loop in IH1.
-      contradiction IH1.
-    + destruct n2 as [|n2].
-  - apply ceval_inf_loop in IH2.
-    contradiction IH2.
-  - destruct (Nat.max_dec (S n1) (S n2)).
-    ** rewrite e. rewrite inline_cseq.
-       apply E_Seq with s'.
-    ++ apply inline_ceval_S with (S n1); [now auto | reflexivity].
-    ++ apply inline_ceval_S with (S n2); [now auto | now apply PeanoNat.Nat.max_l_iff].
-       ** rewrite e. rewrite inline_cseq.
-          apply E_Seq with s'.
-    ++ apply inline_ceval_S with (S n1); [now auto | now apply PeanoNat.Nat.max_r_iff].
-    ++ apply inline_ceval_S with (S n2); [now auto | reflexivity].
-    * exists 2. simpl.  apply E_IfFalse. auto.  apply E_Skip.
-    * destruct IHceval1 as [n1 IH1].
-      destruct IHceval2 as [n2 IH2].
-      exists (S(max n1 n2)).
-      simpl.
-      destruct n1 as [|n1].
-    + apply ceval_inf_loop in IH1.
-      contradiction IH1.
-    + destruct n2 as [|n2].
-  - apply ceval_inf_loop in IH2.
-    contradiction IH2.
-  - destruct (Nat.max_dec (S n1) (S n2)).
-    ** rewrite e.
-       rewrite inline_cif.
-       apply E_IfTrue. assumption.
-       rewrite inline_cseq.
-       apply E_Seq with s'.
-       apply IH1.
-       apply inline_ceval_S with (S n2); [now auto | now apply PeanoNat.Nat.max_l_iff].
-    ** rewrite e.
-       rewrite inline_cif.
-       apply E_IfTrue. assumption.
-       rewrite inline_cseq.
-       apply E_Seq with s'.
-       apply inline_ceval_S with (S n1); [now auto | now apply PeanoNat.Nat.max_r_iff].
-       apply IH2.
-    *  destruct IHceval as [n IH].
-       exists n.
-       destruct n as [|n].
-    + apply ceval_inf_loop in IH.
-      contradiction IH.
-    + rewrite inline_ccall.
-      apply E_Call.
-      apply H.
-Qed.
-
-(** Defintion of a Hoare Triple with inliner for loops **)
-
-Definition i_hoare_triple (n: nat)
-           (P: precondition) (Q: postcondition)
-           (c : com) (ps : Psi.psi) : Prop :=
-  forall s s',  P s -> ceval (k_inliner n c) s ps s'  -> Q s' s.
-
-Lemma i_hoare_triple_hoare_triple :
-  forall P Q p ps,
-    hoare_triple P Q p ps <-> forall n, i_hoare_triple n P Q p ps.
-Proof.
-  unfold hoare_triple, i_hoare_triple;split;intros H.
-  * intros n s s' Pre Heval.
-    eapply H.
-    apply Pre.
-    eapply (inline_n_ceval _ _ _ _ _ Heval).
-  * intros s s' HPre Heval.
-    apply ceval_inline_n in Heval.
-    destruct Heval.
-    eapply (H _ _ _ HPre H0).
+    apply E_IfFalse;[ apply H | apply E_Skip].
+  * specialize (IHceval2 Horig).
+    destruct IHceval2.
+    exists (S x).
+    apply E_IfTrue;[assumption| eapply E_Seq;eauto ]. 
 Qed.
 
 (** Defintion of relational assertion **)
@@ -364,27 +86,27 @@ Definition empty_r_precondition : r_precondition := (fun _ _ => False).
 
 (** Defintion of relational Postcondition **)
 
-Definition r_postcondition : Type :=  sigma -> sigma  -> Prop.
+Definition r_postcondition : Type :=  sigma -> sigma -> sigma -> sigma -> Prop.
 
-Definition empty_r_postcondition :  r_postcondition := (fun _ _ => True).
+Definition empty_r_postcondition :  r_postcondition := (fun _ _ _ _ => True).
 
 (** Definition of quadruple **)
 
 Definition quadruple (P: r_precondition) (Q: r_postcondition)
            (c1 c2: com) (ps : Psi.psi) : Prop :=
-  forall s1 s2 s1' s2', P s1 s2 -> ceval c1 s1 ps s1' -> ceval c2 s2 ps s2' -> Q s1' s2'.
+  forall s1 s2 s1' s2', P s1 s2 -> ceval c1 s1 ps s1' -> ceval c2 s2 ps s2' -> Q s1' s2' s1 s2.
 
 (** Definition of a relational properties with inliner for loops **)
 
 Definition i_quadruple (n: nat) (P: r_precondition) (Q: r_postcondition)
-           (c1 c2 : com) (ps : Psi.psi) : Prop :=
+           (c1 c2 : com) (b1 b2: bexp) (ps : Psi.psi) : Prop :=
   forall s1 s2 s1' s2', P s1 s2 ->
-                   ceval (k_inliner n c1) s1 ps s1' -> ceval (k_inliner n c2) s2 ps s2' ->
-                   Q s1' s2'.
+                   ceval (unroll n b1 c1) s1 ps s1' -> ceval (unroll n b2 c2) s2 ps s2' ->
+                   Q s1' s2' s1 s2.
 
-Lemma qceval_n_inline_loop p1 p2 s1 s2 ps  s1' s2':
-  ceval p1 s1 ps s1' ->  ceval p2 s2 ps s2' ->
-  exists n : nat, ceval (k_inliner n p1) s1 ps s1' /\ ceval (k_inliner n p2) s2 ps s2' .
+Lemma qceval_n_inline_loop b1 b2 p1 p2 s1 s2 inv1 inv2 var1 var2 ps s1' s2':
+  ceval (CWhile b1 p1 inv1 var1) s1 ps s1' ->  ceval (CWhile b2 p2 inv2 var2) s2 ps s2' ->
+  exists n : nat, ceval (unroll n b1 p1) s1 ps s1' /\ ceval (unroll n b2  p2) s2 ps s2' .
 Proof.
   intros Heval1  Heval2.
   apply ceval_inline_n in Heval1.
@@ -394,101 +116,79 @@ Proof.
   * exists x0.
     apply PeanoNat.Nat.max_l_iff in e.
     split.
-    apply (inline_ceval_S _ _ _ _ _ H x0 e).
+    eapply inline_ceval_S;[apply H|assumption].
     apply H0.
   * exists x.
     apply PeanoNat.Nat.max_r_iff in e.
     split.
     apply H.
-    apply (inline_ceval_S _ _ _ _ _ H0 x e).
+    eapply inline_ceval_S;[apply H0|assumption].
 Qed.
 
-Lemma i_quadruple_quadruple P Q p1 p2 ps:
-  quadruple P Q p1 p2 ps <-> forall n, i_quadruple n P Q p1 p2 ps.
+Lemma i_quadruple_quadruple P Q p1 p2 b1 b2 inv1 inv2 var1 var2 ps:
+  quadruple P Q (CWhile b1 p1 inv1 var1) (CWhile b2 p2 inv2 var2) ps
+  <-> forall n, i_quadruple n P Q p1 p2 b1 b2 ps.
 Proof.
   unfold quadruple, i_quadruple;split;intros H.
-  * intros n s1 s2 s1' s2' Pre Heval1 Heval2.
+  - intros n s1 s2 s1' s2' Pre Heval1 Heval2.
     eapply H.
     apply Pre.
-    eapply (inline_n_ceval _  _ _ _ _ Heval1).
-    eapply (inline_n_ceval _  _ _ _ _ Heval2).
-  * intros s1 s2 s1' s2' Pre Heval1 Heval2.
-    specialize (qceval_n_inline_loop _ _ _ _ _ _ _  Heval1 Heval2).
-    intros Heval. destruct Heval as [n Heval]. destruct Heval as (Hevaln1 & Hevaln2).
-    eapply (H n _ _ _ _ Pre Hevaln1 Hevaln2).
+    eapply inline_n_ceval; apply Heval1.
+    eapply inline_n_ceval; apply Heval2.
+  - intros s1 s2 s1' s2' Pre Heval1 Heval2.
+    eapply qceval_n_inline_loop in Heval1; [|apply Heval2].
+    destruct Heval1. destruct H0.
+    eapply H ;eauto.
 Qed.
 
 (** Facts about relational Properties **)
 
 Lemma while_quadruple (inv: r_assertion) b1 b2 c1 c2 ps:
   quadruple (fun s1 s2 => inv s1 s2 /\ beval s1 b1 = true /\ beval s2 b2 =  true)
-            (fun s1' s2' => inv s1' s2' /\ beval s1' b1 = beval s2' b2 ) c1 c2 ps ->
+            (fun s1' s2' _ _ => inv s1' s2' /\ beval s1' b1 = beval s2' b2 ) c1 c2 ps ->
   quadruple ( fun s1 s2 => inv s1 s2 /\ beval s1 b1 = beval s2 b2 )
-            ( fun s1' s2' => inv s1' s2' /\ beval s1' b1 = false /\ beval s2' b2 = false )
-            (CWhile b1 c1 (fun _=> True)) (CWhile b2 c2 (fun _ => True)) ps.
+            ( fun s1' s2' _ _ => inv s1' s2' /\ beval s1' b1 = false /\ beval s2' b2 = false )
+            (CWhile b1 c1 (fun _=> True) (fun _ => 0))
+            (CWhile b2 c2 (fun _ => True) (fun _ => 0)) ps.
 Proof.
   intros Hinv.
   apply i_quadruple_quadruple.
   intros n.
   induction n.
-  * intros s1 s2 s1' s2' HP Heval1 Heval2.
+  - intros s1 s2 s1' s2' HP Heval1 Heval2.
     apply ceval_inf_loop in Heval1.
     contradiction Heval1.
-  * intros s1 s2 s1' s2' HP Heval1 Heval2.
-    rewrite inline_cwhile in Heval1.
-    rewrite inline_cwhile in Heval2.
-    destruct n.
-    apply ceval_inf_loop in Heval1.
-    contradiction Heval1.
-    rewrite inline_cif in Heval1.
-    rewrite inline_cif in Heval2.
-    remember (k_inliner (S n) (CSeq c1 (CWhile b1 c1 (fun _ : list sigma => True)))) as ident.
-    inversion Heval1;clear Heval1;subst.
-  - remember (k_inliner (S n) (CSeq c2 (CWhile b2 c2 (fun _ : list sigma => True)))) as ident.
-    inversion Heval2;clear Heval2; subst.
-    + rewrite inline_cseq in H6.
-      rewrite inline_cseq in H8.
-      remember (k_inliner (S n) (CWhile b1 c1 (fun _ : list sigma => True))) as ident1.
-      remember (k_inliner (S n) c1) as ident2.
-      inversion H6;subst.
-      clear H6.
-      remember (k_inliner (S n) (CWhile b2 c2 (fun _ : list sigma => True))) as ident1.
-      remember (k_inliner (S n) c2) as ident2.
-      inversion H8;subst.
-      clear H8.
-      eapply IHn.
-      eapply Hinv.
-      split. apply HP.
-      split. assumption. assumption.
-      apply inline_n_ceval in H1. apply H1.
-      apply inline_n_ceval in H2. apply H2.
-      assumption. assumption.
-    + destruct HP.
-      rewrite H5 in H0.
-      rewrite H7 in H0.
-      discriminate H0.
-  - remember (k_inliner (S n) (CSeq c2 (CWhile b2 c2 (fun _ : list sigma => True)))) as ident.
-    inversion Heval2;clear Heval2; subst.
-    + destruct HP.
-      rewrite H5 in H0.
-      rewrite H7 in H0.
-      discriminate H0.
-    + inversion H6;subst.
-      inversion H8;subst.
-      split. apply HP.
-      split. assumption. assumption.
+  - intros s1 s2 s1' s2' HP Heval1 Heval2.
+    destruct HP as [HP1 HP2].
+    simpl in Heval1, Heval2.
+    inversion Heval1;subst.
+    + inversion Heval2;subst.
+      * inversion H6;subst.
+        inversion H8;subst.
+        eapply IHn.
+        eapply Hinv.
+        split;[apply HP1 | rewrite H5,H7;auto ].
+        all: try eauto.
+      * rewrite H5,H7 in HP2; now auto.
+    + inversion Heval2;subst.
+      *  rewrite H5,H7 in HP2.
+        inversion HP2.
+      * inversion H6;subst.
+        inversion H8;subst.
+        rewrite H5,H7.
+        auto.
 Qed.
 
 Definition bi_quadruple (i: nat) (P: r_precondition) (Q: r_postcondition)
-           (c1 c2 : com) (ps : Psi.psi) : Prop :=
+           (c1 c2 : com) (b1 b2: bexp) (ps : Psi.psi) : Prop :=
   forall s1 s2 s1' s2' n m , i = n + m -> P s1 s2 ->
-                   ceval (k_inliner n c1) s1 ps s1' ->
-                   ceval (k_inliner m c2) s2 ps s2' ->
-                   Q s1' s2'.
+                   ceval (unroll n b1 c1) s1 ps s1' ->
+                   ceval (unroll m b2 c2) s2 ps s2' ->
+                   Q s1' s2' s1 s2.
 
-Lemma qceval_n_b_inline_loop p1 p2 s1 s2 ps  s1' s2':
-  ceval p1 s1 ps s1' ->  ceval p2 s2 ps s2' ->
-  exists n m: nat, ceval (k_inliner n p1) s1 ps s1' /\ ceval (k_inliner m p2) s2 ps s2' .
+Lemma qceval_n_b_inline_loop p1 p2 b1 b2 inv1 inv2 var1 var2 s1 s2 ps  s1' s2':
+  ceval (CWhile b1 p1 inv1 var1) s1 ps s1' -> ceval (CWhile b2 p2 inv2 var2) s2 ps s2' ->
+  exists n m: nat, ceval (unroll n b1 p1) s1 ps s1' /\ ceval (unroll m b2 p2) s2 ps s2' .
 Proof.
   intros Heval1  Heval2.
   apply ceval_inline_n in Heval1.
@@ -500,23 +200,22 @@ Proof.
   apply H0.
 Qed.
 
-Lemma bi_quadruple_quadruple P Q p1 p2 ps:
-  quadruple P Q p1 p2 ps <-> forall n, bi_quadruple n P Q p1 p2 ps.
+Lemma bi_quadruple_quadruple P Q p1 p2 b1 b2 inv1 inv2 var1 var2 ps:
+  quadruple P Q (CWhile b1 p1 inv1 var1) (CWhile b2 p2 inv2 var2) ps <->
+    forall n, bi_quadruple n P Q p1 p2 b1 b2 ps.
 Proof.
   unfold quadruple, bi_quadruple;split;intros H.
   * intros i s1 s2 s1' s2' n m Hi Pre Heval1 Heval2.
     eapply H.
     apply Pre.
-    eapply (inline_n_ceval _  _ _ _ _ Heval1).
-    eapply (inline_n_ceval _  _ _ _ _ Heval2).
+    eapply inline_n_ceval; apply Heval1.
+    eapply inline_n_ceval; apply Heval2.
   * intros s1 s2 s1' s2' Pre Heval1 Heval2.
-    specialize (qceval_n_b_inline_loop _ _ _ _ _ _ _  Heval1 Heval2).
-    intros Heval. destruct Heval as [n Heval]. destruct Heval as [m Heval].
-    destruct Heval as (Hevaln & Hevalm).
-    specialize (H (n + m) s1 s2 s1' s2' n m).
-    apply H.
+    eapply qceval_n_b_inline_loop in  Heval1; [| apply Heval2].
+    destruct Heval1. destruct H0. destruct H0.
+    eapply (H (x0 + x)).
     reflexivity.
-    assumption.
+    apply Pre.
     assumption.
     assumption.
 Qed.
@@ -559,174 +258,75 @@ Qed.
 Lemma while_skedule_quadruple (inv : r_assertion) (L R : r_cond) b1 b2 c1 c2 ps:
   quadruple (fun s1 s2 => inv s1 s2 /\ beval s1 b1 = true /\ beval s2 b2 = true /\
                          L s1 s2 = false /\ R s1 s2 = false)
-            (fun s1' s2' => inv s1' s2')
+            (fun s1' s2' _ _ => inv s1' s2')
             c1 c2 ps ->
   quadruple (fun s1 s2 => inv s1 s2 /\ beval s1 b1 = true  /\ L s1 s2 = true )
-            (fun s1' s2' => inv s1' s2' )
+            (fun s1' s2' _ _ => inv s1' s2' )
             c1 CSkip ps ->
   quadruple (fun s1 s2 => inv s1 s2 /\ beval s2 b2 = true  /\ R s1 s2 = true)
-            (fun s1' s2' => inv s1' s2')
+            (fun s1' s2' _ _ => inv s1' s2')
             CSkip c2 ps ->
   (forall s1 s2, inv s1 s2 ->
             beval s1 b1 = beval s2 b2 \/
             (beval s1 b1 = true /\ L s1 s2 = true ) \/
             (beval s2 b2 = true /\ R s1 s2 = true)) ->
   quadruple inv
-            ( fun s1' s2' => inv s1' s2' /\ beval s1' b1 = false /\ beval s2' b2 = false )
-            (CWhile b1 c1 (fun _=> True)) (CWhile b2 c2 (fun _ => True)) ps.
+            ( fun s1' s2' _ _ => inv s1' s2' /\ beval s1' b1 = false /\ beval s2' b2 = false )
+            (CWhile b1 c1 (fun _=> True) (fun _ => 0))
+            (CWhile b2 c2 (fun _ => True) (fun _ => 0)) ps.
 Proof.
   intros Hinv1 Hinv2 Hinv3 Hinv.
   apply bi_quadruple_quadruple.
-  intros i.
-  induction i.
-  intros s1 s2 s1' s2' n m Hi HP Heval1 Heval2.
-  symmetry in Hi.
-  apply plus_is_O in Hi.
-  destruct Hi.
-  subst.
-  apply ceval_inf_loop in Heval1.
-  contradiction Heval1.
-  intros s1 s2 s1' s2' n m Hi HP Heval1 Heval2.
-  destruct n.
-  apply ceval_inf_loop in Heval1.
-  contradiction Heval1.
-  destruct m.
-  apply ceval_inf_loop in Heval2.
-  contradiction Heval2.
-  specialize (Hinv _ _ HP).
-  apply simpl_side_condition in Hinv.
-  destruct Hinv.
-  - rewrite inline_cwhile in Heval1.
-    rewrite inline_cwhile in Heval2.
-    destruct n.
-    apply ceval_inf_loop in Heval1.
-    contradiction Heval1.
-    destruct m.
-    apply ceval_inf_loop in Heval2.
-    contradiction Heval2.
-    rewrite inline_cif in Heval1.
-    rewrite inline_cif in Heval2.
-    remember (k_inliner (S n) (CSeq c1 (CWhile b1 c1 (fun _ : list sigma => True)))) as ident.
-    inversion Heval1;clear Heval1;subst.
-    + remember (k_inliner (S m) (CSeq c2 (CWhile b2 c2 (fun _ : list sigma => True)))) as ident.
-      inversion Heval2;clear Heval2; subst.
-      * rewrite inline_cseq in H7.
-        rewrite inline_cseq in H9.
-        remember (k_inliner (S n) (CWhile b1 c1 (fun _ : list sigma => True))) as ident1.
-        remember (k_inliner (S n) c1) as ident2.
-        inversion H7;subst.
-        clear H7.
-        remember (k_inliner (S m) (CWhile b2 c2 (fun _ : list sigma => True))) as ident1.
-        remember (k_inliner (S m) c2) as ident2.
-        inversion H9;subst.
-        clear H9.
-        assert (H12: i = S n + S (S m)) by lia.
-        eapply IHi.
-        apply H12.
-        eapply Hinv1.
-        split. apply HP.
-        assumption.
-        apply inline_n_ceval in H2. apply H2.
-        apply inline_n_ceval in H3. apply H3.
-        assumption.
-        eapply inline_ceval_S.
-        apply H11.
-        lia.
-      * rewrite H6 in H.
-        rewrite H8 in H.
-        decompose [and] H.
-        discriminate H2.
-    + remember (k_inliner (S n) (CSeq c2 (CWhile b2 c2 (fun _ : list sigma => True)))) as ident.
-      inversion Heval2;clear Heval2; subst.
-      * rewrite H6 in H.
-        rewrite H8 in H.
-        decompose [and] H.
-        discriminate H0.
-      * inversion H7;subst.
-        inversion H9;subst.
-        split. apply HP.
-        split. assumption. assumption.
-  - destruct H.
-    + rewrite  inline_cwhile in Heval1.
-      rewrite inline_cwhile in Heval2.
-      destruct n.
-      apply ceval_inf_loop in Heval1.
-      contradiction Heval1.
-      destruct m.
-      apply ceval_inf_loop in Heval2.
-      contradiction Heval2.
-      rewrite inline_cif in Heval1.
-      rewrite inline_cif in Heval2.
-      remember (k_inliner (S n) (CSeq c1 (CWhile b1 c1 (fun _ : list sigma => True)))) as ident.
-      inversion Heval1;clear Heval1;subst.
-      * remember (k_inliner (S m) (CSeq c2 (CWhile b2 c2 (fun _ : list sigma => True)))) as ident.
-        inversion Heval2;clear Heval2; subst.
-        -- rewrite H6 in H.
-           rewrite H8 in H.
-           decompose [and] H.
-           discriminate H0.
-        -- rewrite H6 in H.
-           rewrite H8 in H.
-           decompose [and] H.
-           discriminate H0.
-      * remember (k_inliner (S n) (CSeq c2 (CWhile b2 c2 (fun _ : list sigma => True)))) as ident.
-        inversion Heval2;clear Heval2; subst.
-        -- rewrite H6 in H.
-           rewrite H8 in H.
-           decompose [and] H.
-           discriminate H1.
-        -- inversion H7;subst.
-           inversion H9;subst.
-           split. apply HP.
-           split. assumption. assumption.
+  induction n.
+  - intros s1 s2 s1' s2' n m Hi HP Heval1 Heval2.
+    symmetry in Hi.
+    apply Nat.eq_add_0 in Hi.
+    destruct Hi; subst.
+    apply ceval_inf_loop in Heval1; now auto.
+  - intros s1 s2 s1' s2' n1 n2 Hi HP Heval1 Heval2.
+    destruct n1.
+    apply ceval_inf_loop in Heval1; now auto.
+    destruct n2.
+    apply ceval_inf_loop in Heval2; now auto.
+    specialize (Hinv _ _ HP).
+    apply simpl_side_condition in Hinv.
+    destruct Hinv.
+    + inversion Heval1; subst.
+      inversion Heval2; subst.
+      inversion H7; subst.
+      inversion H9; subst.
+      inversion Hi.
+      eapply IHn ;[ apply H1 | | | ].
+      eapply Hinv1; [ split;[apply HP| apply H] | apply H2 | apply H3].
+      assumption.
+      eapply inline_ceval_S;[apply H12 | Lia.lia].
+      rewrite H8 in H; now auto.
+      rewrite H6 in H; now auto.
     + destruct H.
-      rewrite  inline_cwhile in Heval1.
-      destruct n.
-      apply ceval_inf_loop in Heval1.
-      contradiction Heval1.
-      rewrite inline_cif in Heval1.
-      remember (k_inliner (S n) (CSeq c1 (CWhile b1 c1 (fun _ : list sigma => True)))) as ident.
-      inversion Heval1;clear Heval1;subst.
-      * rewrite inline_cseq in H7.
-        remember (k_inliner (S n) (CWhile b1 c1 (fun _ : list sigma => True))) as ident1.
-        remember (k_inliner (S n) c1) as ident2.
-        inversion H7;subst.
-        clear H7.
-        assert (H12: i = S n + S m) by lia.
-        eapply IHi.
-        apply H12.
-        eapply Hinv2.
-        split. apply HP. assumption.
-        apply inline_n_ceval in H2. apply H2.
-        apply E_Skip.
-        assumption.
-        assumption.
+      * inversion Heval1; subst.
+        rewrite H6 in H; now auto.
+        inversion Heval2; subst.
+        rewrite H8 in H; now auto.
+        inversion H7; subst.
+        inversion H9; subst.
+        auto.
       * destruct H.
-        rewrite H6 in H.
-        discriminate H.
-      * rewrite  inline_cwhile in Heval2.
-        destruct m.
-        apply ceval_inf_loop in Heval2.
-        contradiction Heval2.
-        rewrite inline_cif in Heval2.
-        remember (k_inliner (S m) (CSeq c2 (CWhile b2 c2 (fun _ : list sigma => True)))) as ident.
-        inversion Heval2;clear Heval2;subst.
-        -- rewrite inline_cseq in H7.
-           remember (k_inliner (S m) (CWhile b2 c2 (fun _ : list sigma => True))) as ident1.
-           remember (k_inliner (S m) c2) as ident2.
-           inversion H7;subst.
-           clear H7.
-           assert (H12: i = S n + S m) by lia.
-           eapply IHi.
-           apply H12.
-           eapply Hinv3.
-           split. apply HP. assumption.
-           apply E_Skip.
-           apply inline_n_ceval in H2. apply H2.
+        -- inversion Heval1; subst.
+           inversion H7; subst.
+           inversion Hi.
+           eapply IHn; [ apply H1 | | | ].
+           eapply Hinv2; [split; [apply HP| assumption] | apply H2| apply E_Skip].
+           assumption. assumption.
+           rewrite H6 in H; now auto.
+        -- inversion Heval2; subst.
+           inversion H7; subst.
+           rewrite Nat.add_comm in Hi.
+           inversion Hi.
+           rewrite Nat.add_comm in H1.
+           eapply IHn; [ apply H1 | | | ].
+           eapply Hinv3; [split; [apply HP| assumption] | apply E_Skip | apply H2 ].
            assumption.  assumption.
-        -- destruct H.
-           rewrite H6 in H.
-           discriminate H.
+           rewrite H6 in H; now auto.
 Qed.
 
 (** Definition of a relational contract **)
@@ -775,7 +375,7 @@ Definition bi_quadruple_fun_2 (i: nat) (P: r_precondition) (Q: r_postcondition)
   forall s1 s2 s1' s2' n m, i = n + m -> P s1 s2 ->
                        ceval c1 s1 (k_inliner_ps n ps1) s1' ->
                        ceval c2 s2 (k_inliner_ps m ps2) s2' ->
-                       Q s1' s2'.
+                       Q s1' s2' s1 s2.
 
 Lemma qceval_n_b_inline_fun_2 p1 p2 s1 s2 ps1 ps2 s1' s2':
   ceval p1 s1 ps1 s1' ->  ceval p2 s2 ps2 s2' ->
@@ -793,7 +393,7 @@ Qed.
 
 Definition quadruple_2 (P: r_precondition) (Q: r_postcondition)
            (c1 c2: com) (ps1 ps2 : Psi.psi) : Prop :=
-  forall s1 s2 s1' s2', P s1 s2 -> ceval c1 s1 ps1 s1' -> ceval c2 s2 ps2 s2' -> Q s1' s2'.
+  forall s1 s2 s1' s2', P s1 s2 -> ceval c1 s1 ps1 s1' -> ceval c2 s2 ps2 s2' -> Q s1' s2' s1 s2.
 
 
 Lemma bi_quadruple_quadruple_fun P Q p1 p2 ps1 ps2:
@@ -838,10 +438,11 @@ Definition quadruple_proc_ctx_2 (rcl : R_Phi.r_phi) (ps_init_1 ps_init_2 :Psi.ps
         quadruple_ctx_2 rcl ps1 ps2 (fun s1 s2 => get_r_pre (rcl p1 p2) s1 s2 /\
                                                get_R(rcl p1 p2) s1 s2 = true)
           (get_r_post (rcl p1 p2)) (CCall p1) (ps_init_2 p2)) /\
-    (forall p1 p2 s1 s2,  (get_L(rcl p1 p2) s1 s2 = false /\ get_R(rcl p1 p2) s1 s2 = false) \/
-                       get_L(rcl p1 p2) s1 s2 = true \/ get_R(rcl p1 p2) s1 s2 = true).
+    (forall p1 p2 s1 s2,  get_r_pre (rcl p1 p2) s1 s2 ->
+       ((get_L(rcl p1 p2) s1 s2 = false /\ get_R(rcl p1 p2) s1 s2 = false) \/
+                       get_L(rcl p1 p2) s1 s2 = true \/ get_R(rcl p1 p2) s1 s2 = true)).
 
-Lemma test ps1 ps2 rcl:
+Lemma ext_r_recursive_proc ps1 ps2 rcl:
   quadruple_proc_ctx_2 rcl ps1 ps2 ->
   (forall p1 p2, quadruple_2 (get_r_pre (rcl p1 p2))
               (get_r_post (rcl p1 p2)) (CCall p1) (CCall p2) ps1 ps2).
@@ -854,33 +455,25 @@ Proof.
   induction i.
   intros p1 p2 s1 s2 s1' s2' n m Hi HPre Heval1 Heval2.
   symmetry in Hi.
-  apply plus_is_O in Hi.
-  destruct Hi.
-  subst.
+  apply Nat.eq_add_0 in Hi.
+  destruct Hi; subst.
   inversion Heval1;subst.
-  apply ceval_inf_loop in H1.
-  contradiction H1.
+  apply ceval_inf_loop in H1; now auto.
   intros p1 p2 s1 s2 s1' s2' n m Hi HPre Heval1 Heval2.
   destruct n.
   inversion Heval1;subst.
-  apply ceval_inf_loop in H1.
-  contradiction H1.
+  apply ceval_inf_loop in H1; now auto.
   destruct m.
   inversion Heval2;subst.
-  apply ceval_inf_loop in H1.
-  contradiction H1.
+  apply ceval_inf_loop in H1; now auto.
   unfold quadruple_proc_ctx_2 in H.
   decompose [and] H; clear H.
-  specialize (H4 p1 p2 s1 s2).
+  specialize (H4 p1 p2 s1 s2 HPre).
   destruct H4.
   - eapply H0.
     + intros p0 p3 s0 s1'0 s2'0 s2'1 H5 H6 H7.
       assert (H12: i = n + S m) by lia.
-      eapply IHi.
-      apply H12.
-      apply H5.
-      apply H6.
-      apply H7.
+      eapply IHi;[apply H12|apply H5|apply H6|apply H7].
     + split. apply HPre. apply H.
     + apply n_inline_ps_inline in Heval1.
       apply Heval1.
@@ -891,11 +484,7 @@ Proof.
     + eapply H2.
       * intros p0 p3 s0 s1'0 s2'0 s2'1 H5 H6 H7.
         assert (H12: i = n + S m) by lia.
-        eapply IHi.
-        apply H12.
-        apply H5.
-        apply H6.
-        apply H7.
+        eapply IHi;[apply H12|apply H5|apply H6|apply H7].
       * split. apply HPre. apply H.
       * apply n_inline_ps_inline in Heval1.
         apply Heval1.
@@ -903,21 +492,12 @@ Proof.
     + eapply H1.
       * intros p0 p3 s0 s1'0 s2'0 s2'1 H5 H6 H7.
         assert (H12: i = S n + m) by lia.
-        eapply IHi.
-        apply H12.
-        apply H5.
-        apply H6.
-        apply H7.
+        eapply IHi;[apply H12|apply H5|apply H6|apply H7].
       * split. apply HPre. apply H.
       * apply Heval1.
       * apply n_inline_ps_inline in Heval2.
         apply Heval2.
 Qed.
-
-Definition bi_quadruple_fun (i: nat) (P: r_precondition) (Q: r_postcondition)
-  (c1 c2 : com) (ps : Psi.psi) : Prop :=
-  bi_quadruple_fun_2 i P Q c1 c2 ps ps.
-
 
 Definition quadruple_ctx (rcl:R_Phi.r_phi) (ps: Psi.psi)
   (P: r_precondition) (Q : r_postcondition) (c1 c2:  com) :=
@@ -927,13 +507,19 @@ Definition quadruple_proc_ctx (rcl : R_Phi.r_phi) (ps_init :Psi.psi):=
   quadruple_proc_ctx_2 rcl ps_init ps_init.
 
 Theorem recursion_hoare_triple :
-  forall P Q p1 p2 ps cl,
-    quadruple_proc_ctx cl ps  ->
-    quadruple_ctx cl ps P Q p1 p2 ->
+  forall P Q p1 p2 ps rcl,
+    quadruple_proc_ctx rcl ps  ->
+    quadruple_ctx rcl ps P Q p1 p2 ->
     quadruple P Q p1 p2 ps.
 Proof.
 intros.
 apply H0.
-eapply test.
+eapply ext_r_recursive_proc.
 apply H.
 Qed.
+
+(*Proof the extended rela rule that can use the rule above *)
+
+(*Just use the normal termination for the transitivity application, for
+ partial correction use axiom forall f, s, exit s', call f s s'
+ and proof the rule from the phd*)
